links: add more links axioms for the instructions

CoqOfRust/revm/revm_interpreter/instructions/links/i256.v
@@ -1,7 +1,115 @@
 Require Import CoqOfRust.CoqOfRust.
 Require Import CoqOfRust.links.M.
+Require Import core.links.cmp.
 Require Import revm.links.dependencies.
 Require Import revm.revm_interpreter.instructions.i256.
+
+(*
+pub enum Sign {
+    Minus = -1,
+    Zero = 0,
+    Plus = 1,
+}
+*)
+Module Sign.
+  Inductive t : Set :=
+  | Minus
+  | Zero
+  | Plus.
+
+  Global Instance IsLink : Link t := {
+    Φ := Ty.path "revm_interpreter::instructions::i256::Sign";
+    φ x :=
+      match x with
+      | Minus => Value.StructTuple "revm_interpreter::instructions::i256::Sign::Minus" []
+      | Zero => Value.StructTuple "revm_interpreter::instructions::i256::Sign::Zero" []
+      | Plus => Value.StructTuple "revm_interpreter::instructions::i256::Sign::Plus" []
+      end;
+  }.
+
+  Definition of_ty : OfTy.t (Ty.path "revm_interpreter::instructions::i256::Sign").
+  Proof. eapply OfTy.Make with (A := t); reflexivity. Defined.
+  Smpl Add apply of_ty : of_ty.
+
+  Lemma of_value_with_Minus :
+    Value.StructTuple "revm_interpreter::instructions::i256::Sign::Minus" [] = φ Minus.
+  Proof. reflexivity. Qed.
+  Smpl Add apply of_value_with_Minus : of_value.
+
+  Lemma of_value_with_Zero :
+    Value.StructTuple "revm_interpreter::instructions::i256::Sign::Zero" [] = φ Zero.
+  Proof. reflexivity. Qed.
+  Smpl Add apply of_value_with_Zero : of_value.
+
+  Lemma of_value_with_Plus :
+    Value.StructTuple "revm_interpreter::instructions::i256::Sign::Plus" [] = φ Plus.
+  Proof. reflexivity. Qed.
+  Smpl Add apply of_value_with_Plus : of_value.
+
+  Definition of_value_Minus :
+    OfValue.t (Value.StructTuple "revm_interpreter::instructions::i256::Sign::Minus" []).
+  Proof.
+    econstructor.
+    apply of_value_with_Minus.
+  Defined.
+  Smpl Add apply of_value_Minus : of_value.
+
+  Definition of_value_Zero :
+    OfValue.t (Value.StructTuple "revm_interpreter::instructions::i256::Sign::Zero" []).
+  Proof.
+    econstructor.
+    apply of_value_with_Zero.
+  Defined.
+
+  Definition of_value_Plus :
+    OfValue.t (Value.StructTuple "revm_interpreter::instructions::i256::Sign::Plus" []).
+  Proof.
+    econstructor.
+    apply of_value_with_Plus.
+  Defined.
+  Smpl Add apply of_value_Plus : of_value.
+End Sign.
+
+(* pub fn i256_sign(val: &U256) -> Sign *)
+Instance run_i256_sign (val : Ref.t Pointer.Kind.Ref U256.t) :
+  Run.Trait instructions.i256.i256_sign [] [] [ φ val ] Sign.t.
+Proof.
+  constructor.
+  run_symbolic.
+Admitted.
+
+(* pub fn i256_sign_compl(val: &mut U256) -> Sign *)
+Instance run_i256_sign_compl (val : Ref.t Pointer.Kind.MutRef U256.t) :
+  Run.Trait instructions.i256.i256_sign_compl [] [] [ φ val ] Sign.t.
+Proof.
+  constructor.
+  run_symbolic.
+Admitted.
+
+(* pub fn u256_remove_sign(val: &mut U256) *)
+Instance run_u256_remove_sign (val : Ref.t Pointer.Kind.MutRef U256.t) :
+  Run.Trait instructions.i256.u256_remove_sign [] [] [ φ val ] unit.
+Proof.
+  constructor.
+  run_symbolic.
+Admitted.
+
+(* pub fn two_compl_mut(op: &mut U256) *)
+Instance run_two_compl_mut (op : Ref.t Pointer.Kind.MutRef U256.t) :
+  Run.Trait instructions.i256.two_compl_mut [] [] [ φ op ] unit.
+Proof.
+  constructor.
+  run_symbolic.
+Admitted.
+
+
+(* pub fn i256_cmp(first: &U256, second: &U256) -> Ordering *)
+Instance run_i256_cmp (first second : U256.t) :
+  Run.Trait instructions.i256.i256_cmp [] [] [ φ first; φ second ] Ordering.t.
+Proof.
+  constructor.
+  run_symbolic.
+Admitted.
 
 (* pub fn i256_div(mut first: U256, mut second: U256) -> U256 *)
 Instance run_i256_div (first second : U256.t) :
