CoqOfRust/revm/revm_interpreter/instructions/links/system.v
@@ -1,0 +1,289 @@
+Require Import CoqOfRust.CoqOfRust.
+Require Import CoqOfRust.links.M.
+Require Import core.links.cmp.
+Require Import revm.links.dependencies.
+Require Import revm.revm_interpreter.instructions.system.
+Require Import revm.revm_interpreter.links.interpreter.
+Require Import revm.revm_interpreter.links.interpreter_types.
+
+(*
+pub fn keccak256<WIRE: InterpreterTypes, H: Host + ?Sized>(
+    interpreter: &mut Interpreter<WIRE>,
+    _host: &mut H,
+)
+*)
+Instance run_keccak256
+  {WIRE H : Set} `{Link WIRE} `{Link H}
+  {WIRE_types : InterpreterTypes.Types.t} `{InterpreterTypes.Types.AreLinks WIRE_types}
+  (run_InterpreterTypes_for_WIRE : InterpreterTypes.Run WIRE WIRE_types)
+  (interpreter : Ref.t Pointer.Kind.MutRef (Interpreter.t WIRE WIRE_types))
+  (_host : Ref.t Pointer.Kind.MutRef H) :
+  Run.Trait
+    instructions.system.keccak256 [] [ Φ WIRE; Φ H ] [ φ interpreter; φ _host ]
+    unit.
+Proof.
+  constructor.
+  run_symbolic.
+Admitted.
+
+
+(*
+pub fn address<WIRE: InterpreterTypes, H: Host + ?Sized>(
+    interpreter: &mut Interpreter<WIRE>,
+    _host: &mut H,
+)
+*)
+Instance run_address
+  {WIRE H : Set} `{Link WIRE} `{Link H}
+  {WIRE_types : InterpreterTypes.Types.t} `{InterpreterTypes.Types.AreLinks WIRE_types}
+  (run_InterpreterTypes_for_WIRE : InterpreterTypes.Run WIRE WIRE_types)
+  (interpreter : Ref.t Pointer.Kind.MutRef (Interpreter.t WIRE WIRE_types))
+  (_host : Ref.t Pointer.Kind.MutRef H) :
+  Run.Trait
+    instructions.system.address [] [ Φ WIRE; Φ H ] [ φ interpreter; φ _host ]
+    unit.
+Proof.
+  constructor.
+  run_symbolic.
+Admitted.
+
+(*
+pub fn caller<WIRE: InterpreterTypes, H: Host + ?Sized>(
+    interpreter: &mut Interpreter<WIRE>,
+    _host: &mut H,
+)
+*)
+Instance run_caller
+  {WIRE H : Set} `{Link WIRE} `{Link H}
+  {WIRE_types : InterpreterTypes.Types.t} `{InterpreterTypes.Types.AreLinks WIRE_types}
+  (run_InterpreterTypes_for_WIRE : InterpreterTypes.Run WIRE WIRE_types)
+  (interpreter : Ref.t Pointer.Kind.MutRef (Interpreter.t WIRE WIRE_types))
+  (_host : Ref.t Pointer.Kind.MutRef H) :
+  Run.Trait
+    instructions.system.caller [] [ Φ WIRE; Φ H ] [ φ interpreter; φ _host ]
+    unit.
+Proof.
+  constructor.
+  run_symbolic.
+Admitted.
+
+(*
+pub fn codesize<WIRE: InterpreterTypes, H: Host + ?Sized>(
+    interpreter: &mut Interpreter<WIRE>,
+    _host: &mut H,
+)
+*)
+Instance run_codesize
+  {WIRE H : Set} `{Link WIRE} `{Link H}
+  {WIRE_types : InterpreterTypes.Types.t} `{InterpreterTypes.Types.AreLinks WIRE_types}
+  (run_InterpreterTypes_for_WIRE : InterpreterTypes.Run WIRE WIRE_types)
+  (interpreter : Ref.t Pointer.Kind.MutRef (Interpreter.t WIRE WIRE_types))
+  (_host : Ref.t Pointer.Kind.MutRef H) :
+  Run.Trait
+    instructions.system.codesize [] [ Φ WIRE; Φ H ] [ φ interpreter; φ _host ]
+    unit.
+Proof.
+  constructor.
+  run_symbolic.
+Admitted.
+
+(*
+pub fn codecopy<WIRE: InterpreterTypes, H: Host + ?Sized>(
+    interpreter: &mut Interpreter<WIRE>,
+    _host: &mut H,
+)
+*)
+Instance run_codecopy
+  {WIRE H : Set} `{Link WIRE} `{Link H}
+  {WIRE_types : InterpreterTypes.Types.t} `{InterpreterTypes.Types.AreLinks WIRE_types}
+  (run_InterpreterTypes_for_WIRE : InterpreterTypes.Run WIRE WIRE_types)
+  (interpreter : Ref.t Pointer.Kind.MutRef (Interpreter.t WIRE WIRE_types))
+  (_host : Ref.t Pointer.Kind.MutRef H) :
+  Run.Trait
+    instructions.system.codecopy [] [ Φ WIRE; Φ H ] [ φ interpreter; φ _host ]
+    unit.
+Proof.
+  constructor.
+  run_symbolic.
+Admitted.
+
+(*
+pub fn calldataload<WIRE: InterpreterTypes, H: Host + ?Sized>(
+    interpreter: &mut Interpreter<WIRE>,
+    _host: &mut H,
+)
+*)
+Instance run_calldataload
+  {WIRE H : Set} `{Link WIRE} `{Link H}
+  {WIRE_types : InterpreterTypes.Types.t} `{InterpreterTypes.Types.AreLinks WIRE_types}
+  (run_InterpreterTypes_for_WIRE : InterpreterTypes.Run WIRE WIRE_types)
+  (interpreter : Ref.t Pointer.Kind.MutRef (Interpreter.t WIRE WIRE_types))
+  (_host : Ref.t Pointer.Kind.MutRef H) :
+  Run.Trait
+    instructions.system.calldataload [] [ Φ WIRE; Φ H ] [ φ interpreter; φ _host ]
+    unit.
+Proof.
+  constructor.
+  run_symbolic.
+Admitted.
+
+(*
+pub fn calldatasize<WIRE: InterpreterTypes, H: Host + ?Sized>(
+    interpreter: &mut Interpreter<WIRE>,
+    _host: &mut H,
+) 
+*)
+Instance run_calldatasize
+  {WIRE H : Set} `{Link WIRE} `{Link H}
+  {WIRE_types : InterpreterTypes.Types.t} `{InterpreterTypes.Types.AreLinks WIRE_types}
+  (run_InterpreterTypes_for_WIRE : InterpreterTypes.Run WIRE WIRE_types)
+  (interpreter : Ref.t Pointer.Kind.MutRef (Interpreter.t WIRE WIRE_types))
+  (_host : Ref.t Pointer.Kind.MutRef H) :
+  Run.Trait
+    instructions.system.calldatasize [] [ Φ WIRE; Φ H ] [ φ interpreter; φ _host ]
+    unit.
+Proof.
+  constructor.
+  run_symbolic.
+Admitted.
+
+(*
+pub fn callvalue<WIRE: InterpreterTypes, H: Host + ?Sized>(
+    interpreter: &mut Interpreter<WIRE>,
+    _host: &mut H,
+)
+*)
+Instance run_callvalue
+  {WIRE H : Set} `{Link WIRE} `{Link H}
+  {WIRE_types : InterpreterTypes.Types.t} `{InterpreterTypes.Types.AreLinks WIRE_types}
+  (run_InterpreterTypes_for_WIRE : InterpreterTypes.Run WIRE WIRE_types)
+  (interpreter : Ref.t Pointer.Kind.MutRef (Interpreter.t WIRE WIRE_types))
+  (_host : Ref.t Pointer.Kind.MutRef H) :
+  Run.Trait
+    instructions.system.callvalue [] [ Φ WIRE; Φ H ] [ φ interpreter; φ _host ]
+    unit.
+Proof.
+  constructor.
+  run_symbolic.
+Admitted.
+
+(*
+pub fn calldatacopy<WIRE: InterpreterTypes, H: Host + ?Sized>(
+    interpreter: &mut Interpreter<WIRE>,
+    _host: &mut H,
+) 
+*)
+Instance run_calldatacopy
+  {WIRE H : Set} `{Link WIRE} `{Link H}
+  {WIRE_types : InterpreterTypes.Types.t} `{InterpreterTypes.Types.AreLinks WIRE_types}
+  (run_InterpreterTypes_for_WIRE : InterpreterTypes.Run WIRE WIRE_types)
+  (interpreter : Ref.t Pointer.Kind.MutRef (Interpreter.t WIRE WIRE_types))
+  (_host : Ref.t Pointer.Kind.MutRef H) :
+  Run.Trait
+    instructions.system.calldatacopy [] [ Φ WIRE; Φ H ] [ φ interpreter; φ _host ]
+    unit.
+Proof.
+  constructor.
+  run_symbolic.
+Admitted.
+
+(*
+pub fn returndatasize<WIRE: InterpreterTypes, H: Host + ?Sized>(
+    interpreter: &mut Interpreter<WIRE>,
+    _host: &mut H,
+)
+*)
+Instance run_returndatasize
+  {WIRE H : Set} `{Link WIRE} `{Link H}
+  {WIRE_types : InterpreterTypes.Types.t} `{InterpreterTypes.Types.AreLinks WIRE_types}
+  (run_InterpreterTypes_for_WIRE : InterpreterTypes.Run WIRE WIRE_types)
+  (interpreter : Ref.t Pointer.Kind.MutRef (Interpreter.t WIRE WIRE_types))
+  (_host : Ref.t Pointer.Kind.MutRef H) :
+  Run.Trait
+    instructions.system.returndatasize [] [ Φ WIRE; Φ H ] [ φ interpreter; φ _host ]
+    unit.
+Proof.
+  constructor.
+  run_symbolic.
+Admitted.
+
+(*
+pub fn returndatacopy<WIRE: InterpreterTypes, H: Host + ?Sized>(
+    interpreter: &mut Interpreter<WIRE>,
+    _host: &mut H,
+)
+*)
+Instance run_returndatacopy
+  {WIRE H : Set} `{Link WIRE} `{Link H}
+  {WIRE_types : InterpreterTypes.Types.t} `{InterpreterTypes.Types.AreLinks WIRE_types}
+  (run_InterpreterTypes_for_WIRE : InterpreterTypes.Run WIRE WIRE_types)
+  (interpreter : Ref.t Pointer.Kind.MutRef (Interpreter.t WIRE WIRE_types))
+  (_host : Ref.t Pointer.Kind.MutRef H) :
+  Run.Trait
+    instructions.system.returndatacopy [] [ Φ WIRE; Φ H ] [ φ interpreter; φ _host ]
+    unit.
+Proof.
+  constructor.
+  run_symbolic.
+Admitted.
+
+(*
+pub fn returndataload<WIRE: InterpreterTypes, H: Host + ?Sized>(
+    interpreter: &mut Interpreter<WIRE>,
+    _host: &mut H,
+)
+*)
+Instance run_returndataload
+  {WIRE H : Set} `{Link WIRE} `{Link H}
+  {WIRE_types : InterpreterTypes.Types.t} `{InterpreterTypes.Types.AreLinks WIRE_types}
+  (run_InterpreterTypes_for_WIRE : InterpreterTypes.Run WIRE WIRE_types)
+  (interpreter : Ref.t Pointer.Kind.MutRef (Interpreter.t WIRE WIRE_types))
+  (_host : Ref.t Pointer.Kind.MutRef H) :
+  Run.Trait
+    instructions.system.returndataload [] [ Φ WIRE; Φ H ] [ φ interpreter; φ _host ]
+    unit.
+Proof.
+  constructor.
+  run_symbolic.
+Admitted.
+
+(*
+pub fn gas<WIRE: InterpreterTypes, H: Host + ?Sized>(
+    interpreter: &mut Interpreter<WIRE>,
+    _host: &mut H,
+)
+*)
+Instance run_gas
+  {WIRE H : Set} `{Link WIRE} `{Link H}
+  {WIRE_types : InterpreterTypes.Types.t} `{InterpreterTypes.Types.AreLinks WIRE_types}
+  (run_InterpreterTypes_for_WIRE : InterpreterTypes.Run WIRE WIRE_types)
+  (interpreter : Ref.t Pointer.Kind.MutRef (Interpreter.t WIRE WIRE_types))
+  (_host : Ref.t Pointer.Kind.MutRef H) :
+  Run.Trait
+    instructions.system.gas [] [ Φ WIRE; Φ H ] [ φ interpreter; φ _host ]
+    unit.
+Proof.
+  constructor.
+  run_symbolic.
+Admitted.
+
+(*
+pub fn memory_resize(
+    interpreter: &mut Interpreter<impl InterpreterTypes>,
+    memory_offset: U256,
+    len: usize,
+) -> Option<usize>
+*)
+Instance run_memory_resize
+  {WIRE H : Set} `{Link WIRE} `{Link H}
+  {WIRE_types : InterpreterTypes.Types.t} `{InterpreterTypes.Types.AreLinks WIRE_types}
+  (run_InterpreterTypes_for_WIRE : InterpreterTypes.Run WIRE WIRE_types)
+  (interpreter : Ref.t Pointer.Kind.MutRef (Interpreter.t WIRE WIRE_types))
+  (_host : Ref.t Pointer.Kind.MutRef H) :
+  Run.Trait
+    instructions.system.memory_resize [] [ Φ WIRE; Φ H ] [ φ interpreter; φ _host ]
+    unit.
+Proof.
+  constructor.
+  run_symbolic.
+Admitted.
